Update /dw

dw/DeepWeb/Free/Monad/Common.v
@@ -1,4 +1,4 @@
-(** Common effects *)
+(** More common effects (see [Effect.v] first) *)
 
 (* TODO: make handlers obviously monad morphisms *)
 
@@ -14,122 +14,10 @@ Require Fin.
 From QuickChick Require Show.
 
 Require Import DeepWeb.Free.Monad.Free.
+Require Import DeepWeb.Free.Monad.Internal.
+Require Export DeepWeb.Free.Monad.Effect.
 Import MonadNotations.
-
-Section Extensible.
-
-(** Sums for extensible event types. *)
-
-Definition sum1 (E1 E2 : Type -> Type) (X : Type) : Type :=
-  E1 X + E2 X.
-
-Inductive emptyE : Type -> Type := .
-
-Definition swap1 `(ab : sum1 A B X) : sum1 B A X :=
-  match ab with
-  | inl a => inr a
-  | inr b => inl b
-  end.
-
-Definition bimap_sum1 `(f : A X -> C Y) `(g : B X -> D Y)
-           (ab : sum1 A B X) : sum1 C D Y :=
-  match ab with
-  | inl a => inl (f a)
-  | inr b => inr (g b)
-  end.
-
-(* Automatic application of commutativity and associativity for sums.
-   TODO: This is still quite fragile and prone to
-   infinite instance resolution loops.
- *)
-
-Class Convertible (A B : Type -> Type) :=
-  { convert : forall {X}, A X -> B X }.
-
-(* Don't try to guess. *)
-Global Instance fluid_id A : Convertible A A | 0 :=
-  { convert X a := a }.
-
-(* Destructure sums. *)
-Global Instance fluid_sum `{Convertible A C} `{Convertible B C}
-  : Convertible (sum1 A B) C | 7 :=
-  { convert X ab :=
-      match ab with
-      | inl a => convert a
-      | inr b => convert b
-      end }.
-
-(* Lean left by default for no reason. *)
-Global Instance fluid_left `{Convertible A B} C
-  : Convertible A (sum1 B C) | 8 :=
-  { convert X a := inl (convert a) }.
-
-(* Very incoherent instances. *)
-Global Instance fluid_right `{Convertible A C} B
-  : Convertible A (sum1 B C) | 9 :=
-  { convert X a := inr (convert a) }.
-
-Global Instance fluid_empty A : Convertible emptyE A :=
-  { convert X v := match v with end }.
-
-End Extensible.
-
-Notation "E1 +' E2" := (sum1 E1 E2)
-(at level 50, left associativity) : type_scope.
-
-Notation "E ++' EE" := (List.fold_left sum1 EE E)
-(at level 50, left associativity) : type_scope.
-
-Notation "E -< F" := (Convertible E F)
-(at level 90, left associativity) : type_scope.
-
-Module Import SumNotations.
-
-(* Is this readable? *)
-
-Delimit Scope sum_scope with sum.
-Bind Scope sum_scope with sum1.
-
-Notation "(| x )" := (inr x) : sum_scope.
-Notation "( x |)" := (inl x) : sum_scope.
-Notation "(| x |)" := (inl (inr x)) : sum_scope.
-Notation "( x ||)" := (inl (inl x)) : sum_scope.
-Notation "(| x ||)" := (inl (inl (inr x))) : sum_scope.
-Notation "( x |||)" := (inl (inl (inl x))) : sum_scope.
-Notation "(| x |||)" := (inl (inl (inl (inr x)))) : sum_scope.
-Notation "( x ||||)" := (inl (inl (inl (inl x)))) : sum_scope.
-Notation "(| x ||||)" :=
-  (inl (inl (inl (inl (inr x))))) : sum_scope.
-Notation "( x |||||)" :=
-  (inl (inl (inl (inl (inl x))))) : sum_scope.
-Notation "(| x |||||)" :=
-  (inl (inl (inl (inl (inl (inr x)))))) : sum_scope.
-Notation "( x ||||||)" :=
-  (inl (inl (inl (inl (inl (inl x)))))) : sum_scope.
-Notation "(| x ||||||)" :=
-  (inl (inl (inl (inl (inl (inl (inr x))))))) : sum_scope.
-Notation "( x |||||||)" :=
-  (inl (inl (inl (inl (inl (inl (inl x))))))) : sum_scope.
-
-End SumNotations.
-
-Open Scope sum_scope.
-
-Definition lift {E F X} `{Convertible E F} : M E X -> M F X :=
-  hoist (@convert _ _ _).
-
-Class Embed X Y :=
-  { embed : X -> Y }.
-
-Instance Embed_fun A X Y `{Embed X Y} : Embed (A -> X) (A -> Y) :=
-  { embed := fun x a => embed (x a) }.
-
-Instance Embed_eff E F X `{Convertible E F} : Embed (E X) (M F X) :=
-  { embed := fun e => liftE (convert e) }.
-
-Arguments embed {X Y _} e.
-
-Notation "^ x" := (embed x) (at level 80).
+Import SumNotations.
 
 Definition run {E F X} (run_ : forall Y, F Y -> M E Y)
   : M (E +' F) X -> M E X :=
@@ -173,124 +61,13 @@ Definition choose `{nondetE -< E} `{failureE -< E} {X}
 End NonDeterminism.
 End Basic.
 
-(* Another more flexible and informative variant of [nondetE]
-   (that also incorporates something like [failureE]). *)
 Module NonDeterminismBis.
-  Import List.
-
-  (* Nodes can be of any arity. They are annotated with
-     a string to help debugging. *)
-  Inductive nondetE : Type -> Type :=
-  | Or : forall (n : nat), string -> nondetE (Fin.t n).
-
-  Arguments Or n reason : clear implicits.
-
-  (* [Or] nodes can have no children ([n = 0]), like [failureE]. *)
-  Definition fail {E A} `{nondetE -< E}
-             (reason : string) : M E A :=
-    Vis (convert (Or 0 reason))
-        (fun f => match f : Fin.t 0 with end).
-
-  Fixpoint ix {A} (xs : list A) (i : Fin.t (List.length xs)) : A.
-  Proof.
-    destruct xs as [| x xs']; inversion i as [ | ? i' ].
-    - apply x.
-    - apply (ix _ xs' i').
-  Defined.
-
-  (* Choose one element in a list. *)
-  Definition choose {E A} `{nondetE -< E}
-             (reason : string) (xs : list A) : M E A :=
-    Vis (convert (Or (length xs) reason)) (fun i => Ret (ix xs i)).
-
-  Definition noFinZ {A} (m : Fin.t O) : A := match m with end.
-
-  (* Extend a continuation indexed by [Fin.t] with a new case. *)
-  Definition or_ {E A n} (f1 : M E A) (f2 : Fin.t n -> M E A)
-             (m : Fin.t (S n)) : M E A :=
-    match m in Fin.t n0 return
-          match n0 with
-          | O => False : Type
-          | S n0 => (Fin.t n0 -> Fin.t n)
-          end -> _ with
-    | Fin.F1 => fun _ => f1
-    | Fin.FS m => fun id => f2 (id m)
-    end (fun x => x).
-
-  Definition VisOr {E A n} `{nondetE -< E}
-             (reason : string) (k : Fin.t n -> M E A) :
-    M E A := Vis (convert (Or n reason)) k.
-
-  Notation "'disj' reason ( f1 | .. | fn )" :=
-    (VisOr reason (or_ f1 .. (or_ fn noFinZ) ..))
-  (at level 0, reason at next level) : nondet_scope.
-
-  Notation "'disj' ( f1 | .. | fn )" :=
-    (VisOr "" (or_ f1 .. (or_ fn noFinZ) ..))
-  (at level 0) : nondet_scope.
-
-  Delimit Scope nondet_scope with nondet.
-  Open Scope nondet_scope.
-
-  Example ex_disj : M nondetE nat :=
-    (disj "test" ( ret 0 | ret 1 | ret 2 )).
-
-  Definition or {E A} `{nondetE -< E} (t1 t2 : M E A) : M E A :=
-    disj ( t1 | t2 ).
-
+  Include Effect.NonDeterminism.
   Definition upgrade_or {E A} `{nondetE -< E}
              (e : Basic.nondetE A) : M E A :=
     match e with
     | Basic.Or => or (ret true) (ret false)
     end.
-
-  (* Remove an element from a list, also returning the remaining
-     elements. *)
-
-  (* Helper for [picks]. *)
-  Fixpoint picks' {A} (xs1 xs2 : list A) : list (A * list A) :=
-    match xs2 with
-    | [] => []
-    | x2 :: xs2' =>
-      (x2, rev_append xs1 xs2') :: picks' (x2 :: xs1) xs2'
-    end.
-
-  (* List of ways to pick an element out of a list. *)
-  Definition picks {A} (xs : list A) : list (A * list A) :=
-    picks' [] xs.
-
-  (* [picks] embedded in a tree. *)
-  Definition pick_one {E A} `{nondetE -< E}
-             (reason : string) (xs : list A) : M E (A * list A) :=
-    choose reason (picks xs).
-
-  (* A few helpers for [Fin.t]. *)
-
-  (* A list of [Fin.t]. *)
-  Definition every_fin (m : nat) : list (Fin.t m) :=
-    (fix every_fin m n :=
-       match n return (Fin.t n -> Fin.t m) -> list (Fin.t m) with
-       | O => fun _ => []
-       | S n' => fun k =>
-         k (@Fin.F1 n') :: every_fin m n' (fun i => k (Fin.FS i))
-       end) m m (fun i => i).
-
-  (* Convert a [nat] to a [Fin.t] without too much care. *)
-  Fixpoint to_fin {n : nat} (m : nat) : option (Fin.t n) :=
-    match n, m return option (Fin.t n) with
-    | O, _ => None
-    | S n, O => Some Fin.F1
-    | S n, S m => option_map Fin.FS (to_fin m)
-    end.
-
-  (* Convert a [nat] to a [Fin.t] with even less care. *)
-  Fixpoint to_fin' {n : nat} (m : nat) : Fin.t (S n) :=
-    match n, m return Fin.t (S n) with
-    | O, _ => Fin.F1
-    | S n, O => Fin.F1
-    | S n, S m => Fin.FS (to_fin' m)
-    end.
-
 End NonDeterminismBis.
 
 Section Reader.
